Let $A, B$ and $n$ be integer numbers.
$$
k=A-B
$$
\begin{equation}
F_A F_B=F_{k+1} F_A^2+F_k F_A F_{A-1}
\end{equation}
\begin{equation}
\sum_{i=0}^n F_i^2=F_{n+1} F_n
\end{equation}
\begin{equation}
\sum_{i=0}^n F_i F_{i+1}=F_{n+1}^2-(-1)^n 
\end{equation}
\begin{equation}
    \sum_{i=0}^n F_i F_{i-1}=\sum_{i=0}^{n-1} F_i F_{i+1}
\end{equation}
\begin{equation}
G C D\left(F_m, F_n\right)=F_{G C D(m, n)}
\end{equation}
\begin{equation}
\sum_{0 \leq k \leq n}\left(\begin{array}{c}
n-k \\
k
\end{array}\right)=F i b_{n+1}
\end{equation}
\begin{equation}
\operatorname{gcd}\left(F_n, F_{n+1}\right)=\operatorname{gcd}\left(F_n, F_{n+2}\right)= \operatorname{gcd}\left(F_{n+1}, F_{n+2}\right)=1
\end{equation}
